specify FS operations in terms of link ops

src/FS/FSAPI.v
@@ -6,1107 +6,217 @@ Require Import Relations.Relation_Operators.
 Require Import RelationClasses.
 Require Import Morphisms.
 Require Import Sumbool.
+Require Import FSModel.
 
 Import ListNotations.
 Open Scope string.
 
-(** Declarative spec for a FS interface with concurrent operations, modeled
- after POCS notes.  The file system is represented as set of links.  To allow
- for concurrent operations a directory may contain a link with the same name
- twice, but for different nodes.  For example, we model a rename as a link
- followed by an unlink.  Thus, a lookup after link and before unlink may observe
- a duplicate name, but each name has a different node. *)
 
+(** Opcodes *)
+
+Inductive linkOpT : Type -> Type :=
+| LinkAdd (dir : nat) (name : string) (target : Node) : linkOpT bool
+| LinkAllocFile (dir : nat) (name : string) : linkOpT (option nat)
+| LinkAllocDir (dir : nat) (name : string) : linkOpT (option nat)
+| LinkDel (dir : nat) (name : string) (target : Node) : linkOpT bool
+| LinkLookup (dir : nat) (name : string) : linkOpT (option Node)
+| LinkList (dir : nat) : linkOpT (option (list string))
+| LinkGetRoot : linkOpT nat
+| FileRead (f : nat) : linkOpT string
+| FileWrite (f : nat) (data : string) : linkOpT unit.
 
-(** Data types *)
-
-Inductive Node :=
-| DirNode : forall (dirnum : nat), Node
-| FileNode : forall (filenum : nat), Node
-| SymlinkNode : forall (target : list string), Node.
-
-Record Link := mkLink {
-  LinkFrom : nat;   (* Always a DirNode *)
-  LinkTo : Node;
-  LinkName : string
-}.
-
-Instance Node_equal_dec : EqualDec Node.
-  unfold EqualDec; intros.
-  destruct x, y; try (right; congruence).
-  destruct (eq_nat_dec dirnum dirnum0); subst; eauto.
-    right; congruence.
-  destruct (eq_nat_dec filenum filenum0); subst; eauto.
-    right; congruence.
-  destruct (list_eq_dec string_dec target target0); subst; eauto.
-    right; congruence.
-Defined.
-
-Lemma Link_equal_dec : EqualDec Link.
-  unfold EqualDec; intros.
-  destruct x, y.
-  destruct (eq_nat_dec LinkFrom0 LinkFrom1); subst.
-  destruct (Node_equal_dec LinkTo0 LinkTo1); subst.
-  destruct (string_dec LinkName0 LinkName1); subst.
-  eauto.
-  right; congruence.
-  right; congruence.
-  right; congruence.
-Defined.
-
-Module MDT_Link.
-  Definition t := Link.
-  Definition eq_dec := Link_equal_dec.
-End MDT_Link.
-
-Module Link_as_UDT := Make_UDT(MDT_Link).
-
-Module Graph := MSetWeakList.Make Link_as_UDT.
-
-Definition eq_string (s1 s2 : string) :=
-  if string_dec s1 s2 then true else false.
-
-Definition proper_nameb n : bool := negb (orb (eq_string n  ".") (eq_string n "..")).
-Definition proper_name n := n <> "." /\ n <> "..".
-Definition proper_link l := proper_name (LinkName l).
-Definition proper_links g := Graph.For_all proper_link g.
-Instance proper_proper_link:
-  Proper (eq ==> eq) proper_link.
-Proof.
-  intros ? ?.
-  intros; subst; reflexivity.
-Qed.
-
-Lemma In_add_add_comm: forall a l1 l2 g,
-    Graph.In a (Graph.add l1 (Graph.add l2 g)) ->
-    Graph.In a (Graph.add l2 (Graph.add l1 g)).
-Proof.
-  intros.
-  eapply Graph.add_spec in H; intuition idtac; subst.
-  eapply Graph.add_spec; right. eapply Graph.add_spec; eauto.
-  eapply Graph.add_spec in H0; intuition idtac; subst.
-  eapply Graph.add_spec; eauto.
-  eapply Graph.add_spec; right. eapply Graph.add_spec; eauto.
-Qed.
-
-Definition File := string.
-Definition Files := list File.
-
-Record FS := mkFS {
-  FSRoot : nat;     (* root DirNode *)
-  FSLinks : Graph.t;
-  FSFiles : Files;  (* [filenum]s point into this list *)
-}.
-
-Definition Pathname := list string.
-
-Definition FSEquiv (fs1 fs2 : FS) : Prop :=
-  FSRoot fs1 = FSRoot fs2 /\
-  FSFiles fs1 = FSFiles fs2 /\
-  Graph.Equal (FSLinks fs1) (FSLinks fs2).
-
-Instance FSEquiv_Equiv : Equivalence FSEquiv.
-Proof.
-  split; unfold FSEquiv.
-  - intros f; intuition eauto.
-    reflexivity.
-  - intros f1 f2; intuition eauto.
-    symmetry. eauto.
-  - intros f1 f2 f3; intuition eauto.
-    congruence.
-    congruence.
-    etransitivity; eauto.
-Qed.
-
-Ltac subst_fsequiv :=
-  match goal with
-  | H : FSEquiv ?s1 ?s2 |- _ =>
-    idtac "substituting" s1 "using" H; rewrite H in *; clear H; clear s1;
-    idtac "cleared" s1
-  | H : FSEquiv ?s1 ?s2 |- _ =>
-    idtac "substituting" s2 "using" H; rewrite <- H in *; clear H; clear s2;
-    idtac "cleared" s2
-  end.
-
-(** [path_evaluates] is used to specify lookup *)
-
-Inductive valid_link : forall (fs : FS) (dir : nat) (name : string) (target : Node), Prop :=
-| ValidLink : forall fs dir name target,
-(*
-    proper_name name ->
-    (exists parent name,
-        Graph.In (mkLink parent (DirNode dir) name) (FSLinks fs) ->
-        target <> DirNode parent) ->
-*)
-    Graph.In (mkLink dir target name) (FSLinks fs) ->
-    valid_link fs dir name target
-| ValidDot : forall fs dir,
-    valid_link fs dir "." (DirNode dir)
-| ValidDotDot : forall fs dir name parent,
-    Graph.In (mkLink parent (DirNode dir) name) (FSLinks fs) ->
-    valid_link fs dir ".." (DirNode parent)
-| ValidDotDotRoot : forall fs dir,
-    dir = FSRoot fs ->
-    valid_link fs dir ".." (DirNode dir).
-
-Instance valid_link_proper :
-  Proper (FSEquiv ==> eq ==> eq ==> eq ==> iff) valid_link.
-Proof.
-  intros fs1 fs2 H.
-  intros ? ? ?; subst.
-  intros ? ? ?; subst.
-  intros ? ? ?; subst.
-  unfold FSEquiv in H; intuition idtac.
-  - inversion H1.
-    + eapply ValidLink.
-      eapply H2; eauto.
-    + eapply ValidDot.
-    + eapply ValidDotDot.
-      eapply H2; eauto.
-    + eapply ValidDotDotRoot. congruence.
-  - inversion H1.
-    + eapply ValidLink.
-      eapply H2; eauto.
-    + eapply ValidDot.
-    + eapply ValidDotDot.
-      eapply H2; eauto.
-    + eapply ValidDotDotRoot. congruence.
-Qed.
-
-Definition proper_link' fs l := proper_name (LinkName l) /\
-                             (exists parent, valid_link fs (LinkFrom l) ".." parent ->
-                                (LinkTo l) <> parent).
-
-Inductive path_evaluates : forall (fs : FS) (start : Node) (pn : Pathname) (target : Node), Prop :=
-| PathEvalEmpty : forall fs start,
-  path_evaluates fs start nil start
-| PathEvalFileLink : forall fs startdir name inum,
-  valid_link fs startdir name (FileNode inum)  ->
-  path_evaluates fs (DirNode startdir) ([name]) (FileNode inum)
-| PathEvalDirLink : forall fs startdir name inum pn namenode,
-  valid_link fs startdir name (DirNode inum) ->
-  path_evaluates fs (DirNode inum) pn namenode ->
-  path_evaluates fs (DirNode startdir) (name :: pn) namenode
-| PathEvalSymlink : forall fs startdir name sympath symtarget pn target,
-  valid_link fs startdir name (SymlinkNode sympath) ->
-  path_evaluates fs (DirNode startdir) sympath symtarget ->
-  path_evaluates fs symtarget pn target ->
-  path_evaluates fs (DirNode startdir) (name :: pn) target.
-
-Instance path_evaluates_proper :
-  Proper (FSEquiv ==> eq ==> eq ==> eq ==> iff) path_evaluates.
-Proof.
-  intros fs1 fs2 H.
-  intros ? ? ?; subst.
-  intros ? ? ?; subst.
-  intros ? ? ?; subst.
-  intuition.
-  - induction H0.
-    + eapply PathEvalEmpty.
-    + eapply PathEvalFileLink; eauto.
-      rewrite H in H0. eauto.
-    + eapply PathEvalDirLink; eauto.
-      rewrite H in H0. eauto.
-    + eapply PathEvalSymlink; eauto.
-      rewrite H in H0; eauto.
-  - induction H0.
-    + eapply PathEvalEmpty.
-    + eapply PathEvalFileLink; eauto.
-      rewrite <- H in H0. eauto.
-    + eapply PathEvalDirLink; eauto.
-      rewrite <- H in H0. eauto.
-    + eapply PathEvalSymlink; eauto.
-      rewrite <- H in H0; eauto.
-Qed.
-
-Definition path_eval_root (fs : FS) (pn : Pathname) (target : Node) : Prop :=
-  path_evaluates fs (DirNode (FSRoot fs)) pn target.
-
-Instance path_eval_root_proper :
-  Proper (FSEquiv ==> eq ==> eq ==> iff) path_eval_root.
-Proof.
-  intros fs1 fs2 H.
-  intros ? ? ?; subst.
-  intros ? ? ?; subst.
-  unfold path_eval_root.
-  eapply path_evaluates_proper; eauto.
-  unfold FSEquiv in *; intuition.
-Qed.
-
-Hint Constructors valid_link.
-Hint Constructors path_evaluates.
-
-Lemma path_evaluates_cons': forall fs startdir name pn node,
-    path_evaluates fs startdir (name::pn) node ->
-    exists node',
-      path_evaluates fs startdir [name] node' /\
-      path_evaluates fs node' pn node.
-Proof.
-  intros.
-  inversion H; subst; eexists; eauto.
-Qed.
-
-Lemma path_evaluates_cons: forall fs startdir name pn node node',
-    path_evaluates fs (DirNode startdir) [name] node' ->
-    path_evaluates fs node' pn node ->
-    exists node'',
-      path_evaluates fs (DirNode startdir) (name::pn) node''.
-Proof.
-  intros.
-  inversion H; subst; clear H.
-  - eexists.
-    inversion H0; subst; clear H0.
-    constructor; eauto.
-  - eexists.
-    eapply PathEvalDirLink; eauto.
-    inversion H7; subst; clear H7.
-    eauto.
-  - eexists.
-    inversion H8; subst; clear H8.
-    eapply PathEvalSymlink; eauto.
-Qed.
-
-Definition does_not_exist (fs : FS) dirnum name :=
-  ~ exists n, Graph.In (mkLink dirnum n name) (FSLinks fs).
-
-Definition file_handle_unused (fs : FS) h :=
-  ~ exists d name, Graph.In (mkLink d (FileNode h) name) (FSLinks fs).
-
-Definition file_handle_valid (fs : FS) h :=
-  h < Datatypes.length (FSFiles fs).
-
-Definition upd_file h data (fs : FS) :=
-  mkFS (FSRoot fs) (FSLinks fs) (list_upd (FSFiles fs) h data).
-
-Definition add_link dir node name (fs : FS) :=
-  mkFS (FSRoot fs) (Graph.add (mkLink dir node name) (FSLinks fs)) (FSFiles fs).
-
-Definition create_file dir h name (fs : FS) :=
-  add_link dir (FileNode h) name (upd_file h "" fs).
-
-Definition valid_dir dir (fs : FS) :=
-  exists pn, path_eval_root fs pn (DirNode dir).
-
-(* If pn exists, then it is unique. *)
-Definition unique_pathname (fs : FS) startdir pn :=
-  exists node,
-    path_evaluates fs startdir pn node /\
-    forall node',
-      path_evaluates fs startdir pn node' -> node' = node.
-
-Definition unique_pathname_root (fs : FS) pn :=
-  exists node,
-    path_eval_root fs pn node /\
-    forall node',
-      path_eval_root fs pn node' -> node' = node.
-
-Lemma unique_pathname_path_evaluates_eq: forall fs startdir pn node node',
-    unique_pathname fs startdir pn ->
-    path_evaluates fs startdir pn node ->
-    path_evaluates fs startdir pn node' ->
-    node = node'.
-Proof.
-  intros.
-  unfold unique_pathname in *.
-  deex.
-  specialize (H2 node H0) as H2x; subst.
-  specialize (H2 node' H1) as H2x; subst.
-  reflexivity.
-Qed.
-
-Lemma unique_pathname_valid_link_eq: forall fs dirnum name inum inum',
-    unique_pathname fs (DirNode dirnum) [name] ->
-    valid_link fs dirnum name (DirNode inum) ->
-    valid_link fs dirnum name (DirNode inum') ->
-    DirNode inum = DirNode inum'.
-Proof.
-  intros.
-  unfold unique_pathname in *.
-  deex.
-  specialize (H2 (DirNode inum)) as H2x; subst.
-  specialize (H2 (DirNode inum')) as H2y; subst.
-  destruct H2x.
-  econstructor.
-  eapply H0.
-  constructor.
-  destruct H2y.
-  econstructor.
-  eapply H1.
-  constructor.
-  reflexivity.
-Qed.
-
-Lemma unique_pathname_path_evaluates_cons_eq: forall fs startdir name pn' node node' node'',
-    path_evaluates fs (DirNode startdir) [name] node' ->
-    path_evaluates fs node' pn' node ->
-    unique_pathname fs (DirNode startdir) [name] ->
-    unique_pathname fs node' pn' ->
-    path_evaluates fs (DirNode startdir) (name :: pn') node'' ->
-    node = node''.
-Proof.
-  intros.
-  eapply path_evaluates_cons' in H3 as Hcons.
-  deex.
-  assert (node'0 = node').
-  eapply unique_pathname_path_evaluates_eq in H; eauto.
-  subst.
-  assert (node = node'').
-  eapply unique_pathname_path_evaluates_eq in H2; eauto.
-  subst.
-  reflexivity.
-Qed.
-
-(* A stronger version of unique_pathname, requiring all intermediate nodes match *)
-Inductive stable_pathname : forall (fs: FS) (startdir: Node) (pn: Pathname), Prop :=
-| StablePathNil: forall fs startdir, stable_pathname fs (DirNode startdir) []
-| StablePathCons: forall fs startdir name pn' node node',
-    path_evaluates fs (DirNode startdir) [name] node' ->
-    path_evaluates fs node' pn' node ->
-    unique_pathname fs (DirNode startdir) [name] ->
-    unique_pathname fs node' pn' ->
-    stable_pathname fs (DirNode startdir) (name::pn').
-
-(* sanity check *)
-Lemma stable_pathname_unique_pathname: forall fs startdir pn,
-    stable_pathname fs startdir pn ->
-    unique_pathname fs startdir pn.
-Proof.
-  intros.
-  inversion H; subst; clear H.
-  - eexists.
-    split.
-    constructor.
-    intros.
-    inversion H; auto.
-  - unfold unique_pathname.
-    eapply path_evaluates_cons in H1 as Hcons; eauto.
-    deex.
-    eapply unique_pathname_path_evaluates_cons_eq in H as Hx; eauto.
-    subst.
-    exists node''.
-    split; eauto.
-    intros.
-    eapply unique_pathname_path_evaluates_cons_eq in H4 as Hx; eauto.
-Qed.
-                               
-Definition unique_dirent (fs : FS) dir name :=
-  forall target target0,
-    valid_link fs dir name target ->
-    valid_link fs dir name target0 ->
-    target0 = target.
-
-Definition unique_dirents (fs : FS) :=
-  forall dir name target target0,
-    valid_link fs dir name target ->
-    valid_link fs dir name target0 ->
-    target0 = target.
-
-Lemma unique_dirent_link_eq: forall fs startdir name node node',
-    unique_dirent fs startdir name ->
-    valid_link fs startdir name node ->
-    valid_link fs startdir name node' ->
-    node = node'.
-Proof.
-  intros.
-  edestruct H; eauto.
-Qed.
-
-(* . and .. are unique; which we get from definition.
-  no other name in directory refers to parent or cur directory *)
-
-Definition fs_invariant (fs : FS) := proper_links (FSLinks fs).
-
-(*
-Definition unique_dotdot (fs : FS) :=
-
-                  
-Definition fs_invariant1 (fs : FS) := proper_links (FSLinks fs) /\
-                                      unique_dotdot.
-*)
-
-Lemma fs_invariant_proper_name: forall fs startdir node name,
-    fs_invariant fs ->
-    Graph.In (mkLink startdir node name) (FSLinks fs) ->
-    proper_name name.
-Proof.
-  intros.
-  unfold fs_invariant in *.
-  unfold proper_links in *.
-  unfold Graph.For_all in *.
-  specialize (H (mkLink startdir node name) H0); eauto.
-Qed.
-
-Lemma fs_invariant_add_link: forall fs dirnum name node,
-    fs_invariant fs ->
-    proper_name name ->
-    does_not_exist fs dirnum name ->
-    fs_invariant (add_link dirnum node name fs).
-Proof.
-  intros.
-  unfold fs_invariant in *.
-  unfold proper_links in *.
-  unfold proper_link in *.
-  unfold Graph.For_all in *.
-  intros; simpl in *.
-  eapply Graph.add_spec in H2; eauto.
-  intuition idtac; subst; simpl in *; eauto.
-Qed.
-
-Lemma path_evaluates_add_link : forall fs startdir dirnum name dirpn n node,
-  path_evaluates fs startdir dirpn node ->
-  path_evaluates (add_link dirnum n name fs) startdir dirpn node.
-Proof.
-  unfold add_link in *.
-  simpl in *.
-  intros.
-  induction H.
-  + constructor.
-  + eapply PathEvalFileLink; eauto.
-    edestruct H.
-    - constructor; simpl.
-      apply Graph.add_spec; auto.
-    - apply ValidDot.
-    - eapply ValidDotDot.
-      apply Graph.add_spec; auto.
-      right; eauto.
-    - apply ValidDotDotRoot; auto.
-  + eapply PathEvalDirLink; eauto.
-    edestruct H.
-    - constructor; simpl.
-      apply Graph.add_spec; auto.
-    - apply ValidDot.
-    - eapply ValidDotDot.
-      apply Graph.add_spec; auto.
-      right; eauto.
-    - apply ValidDotDotRoot; auto.
-  + inversion H; subst.
-    eapply PathEvalSymlink; simpl.
-    - constructor.
-      apply Graph.add_spec.
-      eauto.
-    - apply IHpath_evaluates1; eauto.
-    - apply IHpath_evaluates2; eauto.
-Qed.
-
-Lemma valid_link_does_not_exist: forall fs dirnum name node,
-    proper_name name ->
-    valid_link fs dirnum name node ->
-    does_not_exist fs dirnum name ->
-    False.
-Proof.
-  intros.
-  inversion H0; subst; clear H0.
-  - destruct H1; eexists; eauto.
-  - destruct H; congruence.
-  - destruct H; congruence.
-  - destruct H; congruence.
-Qed.
-
-Lemma path_evaluates_does_not_exist: forall fs dirnum name,
-    proper_name name ->
-    path_evaluates fs (DirNode dirnum) [name] (DirNode dirnum) ->
-    does_not_exist fs dirnum name ->
-    False.
-Proof.
-  intros.
-  inversion H0; subst; clear H0.
-  inversion H8; subst; clear H8.
-  eapply valid_link_does_not_exist; eauto.
-  inversion H9; subst; clear H9.
-  eapply valid_link_does_not_exist; eauto.
-Qed.
-
-Lemma valid_link_add_link': forall fs startdir name name0 dirnum n node node',
-    proper_name name0 ->
-    valid_link fs startdir name0 node ->
-    proper_name name  ->
-    does_not_exist fs dirnum name ->
-    valid_link (add_link dirnum n name fs) startdir name0 node' ->
-    valid_link fs startdir name0 node'.
-Proof.
-  intros.
-  inversion H3; subst; clear H3.
-  - apply Graph.add_spec in H4.
-    intuition idtac; auto.
-    inversion H3; subst; clear H3.
-    exfalso; eapply valid_link_does_not_exist; eauto.
-  - apply ValidDot.
-  - eapply ValidDotDot.
-    apply Graph.add_spec in H4; auto.
-    intuition idtac; eauto.
-    inversion H3; subst. clear H3.
-    inversion H; congruence.
-  - eapply ValidDotDotRoot.
-    simpl in *.
-    reflexivity.
-Qed. 
-
-Lemma valid_link_add_link'': forall fs startdir name name0 dirnum n node node',
-    valid_link fs startdir name0 node ->
-    proper_name name  ->
-    does_not_exist fs dirnum name ->
-    valid_link (add_link dirnum n name fs) startdir name0 node' ->
-    valid_link fs startdir name0 node'.
-Proof.
-  intros.
-  inversion H2; subst; clear H2.
-  - apply Graph.add_spec in H3.
-    intuition idtac; auto.
-    inversion H2; subst; clear H2.
-    exfalso; eapply valid_link_does_not_exist; eauto.
-  - apply ValidDot.
-  - eapply ValidDotDot.
-    apply Graph.add_spec in H3; auto.
-    intuition idtac; eauto.
-    inversion H2; subst. clear H2.
-    admit. 
-  - eapply ValidDotDotRoot.
-    simpl in *.
-    reflexivity.
-Admitted. 
-
-Lemma path_evaluates_add_link' : forall fs startdir dirnum name dirpn n node,
-  fs_invariant fs ->
-  stable_pathname fs startdir dirpn ->
-  path_evaluates fs startdir dirpn (DirNode dirnum) ->
-  does_not_exist fs dirnum name  ->
-  proper_name name ->
-  path_evaluates (add_link dirnum n name fs) startdir dirpn node ->
-  path_evaluates fs startdir dirpn node.
-Proof.
-  intros.
-  remember (add_link dirnum n name fs).
-  generalize dependent fs; intros.
-  induction H4; subst.
-  - constructor.
-  - eapply PathEvalFileLink; subst; eauto.
-    inversion H4; subst.
-    eapply fs_invariant_proper_name in H5 as H5x.
-    eapply Graph.add_spec in H5.
-    intuition idtac.
-    + inversion H6; subst; clear H6.
-      eapply path_evaluates_does_not_exist in H2; eauto.
-      exfalso; auto.
-    + constructor; eauto.
-    + apply fs_invariant_add_link; eauto.
-  - inversion H1; subst; clear H1.
-    {
-      eapply PathEvalDirLink; eauto.
-      eapply valid_link_add_link'' in H4; auto.
-      assert (DirNode inum0 = DirNode inum).
-      {
-        inversion H0; subst.
-        eapply unique_pathname_valid_link_eq.
-        eapply H13.
-        eauto.
-        eauto.
-      }
-      inversion H1; subst; clear H1.
-      eapply IHpath_evaluates; eauto.
-      admit.
-      eauto.
-    }
-    {
-      inversion H10; subst.
-      eapply fs_invariant_proper_name in H1 as Hx; eauto.
-      eapply valid_link_add_link'' in H4; eauto.
-      exfalso. admit. (* H2 + H8 + H *)
-    }
-  - eapply PathEvalSymlink; eauto; subst.
-    inversion H0; subst.
-    (*
-    - constructor.
-      apply Graph.add_spec.
-      eauto.
-    - apply IHpath_evaluates1; eauto.
-    - apply IHpath_evaluates2; eauto.
-*)
-Admitted.
-
-Lemma path_eval_root_add_link : forall fs dirnum name dirpn n,
-  path_eval_root fs dirpn (DirNode dirnum) ->
-  path_eval_root (add_link dirnum n name fs) dirpn (DirNode dirnum).
-Proof.
-  intros.
-  unfold path_eval_root.
-  eapply path_evaluates_add_link in H; eauto.
-Qed.
-
-Lemma path_evaluates_upd_file : forall fs startdir dirnum h data dirpn,
-  path_evaluates fs startdir dirpn (DirNode dirnum) ->
-  path_evaluates (upd_file h data fs) startdir dirpn (DirNode dirnum).
-Proof.
-  intros.
-  unfold upd_file; simpl.
-  induction H.
-  + constructor.
-  + eapply PathEvalFileLink; eauto.
-    edestruct H.
-    - constructor; simpl; auto.
-    - apply ValidDot.
-    - eapply ValidDotDot; simpl; eauto.
-    - apply ValidDotDotRoot; auto.
-  + eapply PathEvalDirLink; eauto.
-    edestruct H.
-    - constructor; simpl; auto.
-    - apply ValidDot.
-    - eapply ValidDotDot; simpl; eauto.
-    - apply ValidDotDotRoot; auto.
-  + eapply PathEvalSymlink; simpl.
-    inversion H. constructor. eauto.
-    apply IHpath_evaluates1; eauto.
-    apply IHpath_evaluates2; eauto.
-Qed.
-
-Lemma path_eval_root_upd_file : forall fs dirnum h data dirpn,
-  path_eval_root fs dirpn (DirNode dirnum) ->
-  path_eval_root (upd_file h data fs) dirpn (DirNode dirnum).
-Proof.
-  intros.
-  unfold path_eval_root in *.
-  eapply path_evaluates_upd_file in H; eauto.
-Qed.
-
-Lemma path_evaluates_upd_file' : forall fs node h data dirpn startdir,
-  path_evaluates (upd_file h data fs) startdir dirpn node ->
-  path_evaluates fs startdir dirpn node.
-Proof.
-  intros.
-  match goal with
-  | H : path_evaluates ?fs0 ?dir0 ?pn0 ?node0 |- _ =>
-    remember fs0;
-    induction H; intros; subst; simpl
-  end.
-  + constructor.
-  + eapply PathEvalFileLink; eauto.
-    inversion H; clear H; subst.
-    constructor. eauto.
-  + eapply PathEvalDirLink; eauto.
-    inversion H; clear H; subst.
-    - constructor. eauto.
-    - apply ValidDot.
-    - eapply ValidDotDot; simpl; eauto.
-    - apply ValidDotDotRoot; auto.
-  + eapply PathEvalSymlink; simpl.
-    inversion H; clear H; subst.
-    constructor; eauto.
-    eapply IHpath_evaluates1; eauto.
-    apply IHpath_evaluates2; eauto.
-Qed.
-
-Lemma path_eval_root_upd_file' : forall fs node h data dirpn,
-  path_eval_root (upd_file h data fs) dirpn node ->
-  path_eval_root fs dirpn node.
-Proof.
-  intros.
-  eapply path_evaluates_upd_file'; eauto.
-Qed.
-
-Lemma does_not_exist_add_link : forall fs dirnum name dirnum0 n0 name0,
-  does_not_exist (add_link dirnum0 n0 name0 fs) dirnum name ->
-  does_not_exist fs dirnum name.
-Proof.
-  intros.
-  unfold does_not_exist, add_link in *.
-  simpl in *.
-  intro.
-  destruct H.
-  deex.
-  eexists.
-  apply Graph.add_spec. right.
-  apply H.
-Qed.
-  
-Lemma does_not_exist_add_link_same_dirnum : forall fs dirnum name n0 name0,
-  does_not_exist fs dirnum name ->
-  name <> name0 ->
-  does_not_exist (add_link dirnum n0 name0 fs) dirnum name.
-Proof.
-  intros.
-  unfold does_not_exist, add_link in *.
-  simpl in *.
-  intro.
-  deex.
-  apply Graph.add_spec in H1.
-  intuition idtac.
-  inversion H2; congruence.
-  destruct H.
-  eexists.
-  apply H2.
-Qed.
-  
-Lemma does_not_exist_upd_file : forall fs h data dirnum name,
-  does_not_exist (upd_file h data fs) dirnum name ->
-  does_not_exist fs dirnum name.
-Proof.
-  intros.
-  unfold does_not_exist, upd_file in *.
-  simpl in *; auto.
-Qed.
-
-Lemma does_not_exist_upd_file' : forall fs h data dirnum name,
-  does_not_exist fs dirnum name ->
-  does_not_exist (upd_file h data fs) dirnum name.
-Proof.
-  intros.
-  unfold does_not_exist, upd_file in *.
-  simpl in *; auto.
-Qed.
-  
-Hint Resolve does_not_exist_add_link.
-Hint Resolve does_not_exist_add_link_same_dirnum.
-Hint Resolve does_not_exist_upd_file.
-Hint Resolve does_not_exist_upd_file'.
-
-Lemma file_handle_unused_upd_file : forall fs h0 data0 h,
-  file_handle_unused (upd_file h0 data0 fs) h ->
-  file_handle_unused fs h.
-Proof.
-  intros.
-  unfold file_handle_unused, upd_file in *.
-  simpl in *; auto.
-Qed.
-
-Lemma file_handle_unused_add_link : forall fs dirnum n name h,
-  file_handle_unused (add_link dirnum n name fs) h ->
-  file_handle_unused fs h.
-Proof.
-  intros.
-  unfold file_handle_unused, add_link in *.
-  simpl in *.
-  intro.
-  repeat deex.
-  destruct H.
-  repeat eexists.
-  apply Graph.add_spec.
-  right. apply H0.
-Qed.
-  
-Lemma file_handle_unused_upd_file' : forall fs h0 data0 h,
-  file_handle_unused fs h ->
-  file_handle_unused (upd_file h0 data0 fs) h.
-Proof.
-  intros.
-  unfold file_handle_unused, upd_file in *.
-  simpl in *; auto.
-Qed.
-
-Lemma file_handle_unused_add_link' : forall fs dirnum n name h,
-  file_handle_unused fs h ->
-  n <> FileNode h ->
-  file_handle_unused (add_link dirnum n name fs) h.
-Proof.
-  intros.
-  unfold file_handle_unused, add_link in *.
-  simpl in *.
-  intro.
-  repeat deex.
-  apply Graph.add_spec in H1.
-  intuition idtac.
-  inversion H2; congruence.
-  destruct H.
-  repeat eexists.
-  apply H2.
-Qed.
-  
-Lemma file_handle_unused_ne : forall fs dirnum v0 v1 name,
-  file_handle_unused (add_link dirnum (FileNode v0) name fs) v1 ->
-  FileNode v1 <> FileNode v0.
-Proof.
-  intros.
-  unfold file_handle_unused, add_link in *.
-  simpl in *.
-  intro.
-  destruct H.
-  repeat eexists.
-  apply Graph.add_spec.
-  left. rewrite H0; eauto.
-Qed.
-
-Hint Resolve file_handle_unused_upd_file.
-Hint Resolve file_handle_unused_add_link.
-Hint Resolve file_handle_unused_add_link'.
-Hint Resolve file_handle_unused_ne.
-
-Lemma file_handle_valid_upd_file : forall fs h0 data0 h,
-  file_handle_valid (upd_file h0 data0 fs) h ->
-  file_handle_valid fs h.
-Proof.
-  intros.
-  unfold file_handle_valid, file_handle_valid, upd_file in *.
-  simpl in *.
-  rewrite length_list_upd in H; auto.
-Qed.
-
-Lemma file_handle_valid_add_link : forall fs dirnum n name h,
-  file_handle_valid (add_link dirnum n name fs) h ->
-  file_handle_valid fs h.
-Proof.
-  intros.
-  unfold file_handle_valid, file_handle_valid, add_link in *.
-  simpl in *; auto.
-Qed.
-
-Lemma file_handle_valid_upd_file' : forall fs h0 data0 h,
-  file_handle_valid fs h ->
-  file_handle_valid (upd_file h0 data0 fs) h.
-Proof.
-  intros.
-  unfold file_handle_valid, file_handle_valid, upd_file in *.
-  simpl in *.
-  rewrite length_list_upd; auto.
-Qed.
-  
-Lemma file_handle_valid_add_link' : forall fs dirnum n name h,
-  file_handle_valid fs h ->
-  file_handle_valid (add_link dirnum n name fs) h.
-Proof.
-  intros.
-  unfold file_handle_valid, file_handle_valid, add_link in *.
-  simpl in *; auto.
-Qed.
-  
-Hint Resolve file_handle_valid_upd_file.
-Hint Resolve file_handle_valid_add_link.
-Hint Resolve file_handle_valid_upd_file'.
-Hint Resolve file_handle_valid_add_link'.
-
-Lemma valid_link_upd_file' : forall fs h data dir name target,
-  valid_link (upd_file h data fs) dir name target ->
-  valid_link fs dir name target.
-Proof.
-  intros.
-  remember (upd_file h data fs); generalize dependent fs.
-  induction H; intros; subst.
-  - constructor. eauto.
-  - eapply ValidDot.
-  - eapply ValidDotDot. eauto.
-  - eapply ValidDotDotRoot. eauto.
-Qed.
-
-(* File system operations *)
 
 Inductive stat_result :=
-| StatMissing
 | StatFile
 | StatDir.
 
 Inductive fsOpT : Type -> Type :=
-| Create (dir : Pathname) (name : string) : fsOpT nat
-| Mkdir (dir : Pathname) (name : string) : fsOpT nat
-| Delete (pn : Pathname) : fsOpT unit
-| Rmdir (pn : Pathname) : fsOpT unit
-| Stat (dir : Pathname) (name : string) : fsOpT stat_result
-| Readdir (pn : Pathname) : fsOpT (list string)
-| Rename (src : Pathname) (dstdir : Pathname) (dstname : string) : fsOpT unit
-| Read (pn : Pathname) : fsOpT string
-| Write (pn : Pathname) (data : string) : fsOpT unit
-| FindAvailableName (dir : Pathname) : fsOpT string
+| Create (cwd : nat) (dir : Pathname) (name : string) : fsOpT nat
+| Mkdir (cwd : nat) (dir : Pathname) (name : string) : fsOpT nat
+| Unlink (cwd : nat) (dir : Pathname) (name : string) : fsOpT unit
+| Stat (cwd : nat) (dir : Pathname) (name : string) : fsOpT (option stat_result)
+| Readdir (cwd : nat) (pn : Pathname) : fsOpT (list string)
+| Rename (cwd : nat) (src : Pathname) (dstdir : Pathname) (dstname : string) : fsOpT unit
+| Read (cwd : nat) (pn : Pathname) : fsOpT string
+| Write (cwd : nat) (pn : Pathname) (data : string) : fsOpT unit
+| FindAvailableName (cwd : nat) (dir : Pathname) : fsOpT string
 | Debug (s : string) : fsOpT unit.
 
 
-(* Semantics of file system operations *)
+Module LinkAPI <: Layer.
 
-Definition State := FS.
+  Definition opT := linkOpT.
+  Definition State := FS.
 
-Section StepXform.
+  Inductive xstep : forall T, opT T -> nat -> State -> T -> State -> Prop :=
+  | StepAdd : forall dir name target tid fs,
+    xstep (LinkAdd dir name target) tid
+      fs
+      true
+      (add_link dir target name fs)
+  | StepAllocFile : forall dir name fid tid fs,
+    file_handle_valid fs fid ->
+    file_handle_unused fs fid ->
+    xstep (LinkAllocFile dir name) tid
+      fs
+      (Some fid)
+      (add_link dir (FileNode fid) name fs)
+  | StepAllocDir : forall dir name did tid fs,
+    (~ exists pn, path_eval_root fs pn (DirNode did)) ->
+    xstep (LinkAllocDir dir name) tid
+      fs
+      (Some did)
+      (add_link dir (DirNode did) name fs)
+  | StepDel : forall dir name target tid fs,
+    xstep (LinkDel dir name target) tid
+      fs
+      true
+      (del_link dir target name fs)
+  | StepLookupAbsent : forall dir name tid fs,
+    (~ exists target, valid_link fs dir name target) ->
+    xstep (LinkLookup dir name) tid
+      fs
+      None
+      fs
+  | StepLookupFound : forall dir name target tid fs,
+    valid_link fs dir name target ->
+    xstep (LinkLookup dir name) tid
+      fs
+      (Some target)
+      fs
+  | StepList : forall dir tid fs,
+    xstep (LinkList dir) tid
+      fs
+      (Some (readdir_names fs dir))
+      fs
+  | StepGetRoot : forall tid fs,
+    xstep LinkGetRoot tid
+      fs
+      (FSRoot fs)
+      fs
+  | StepRead : forall f data tid fs,
+    nth_error (FSFiles fs) f = Some data ->
+    xstep (FileRead f) tid
+      fs
+      data
+      fs
+  | StepWrite : forall f data tid fs,
+    xstep (FileWrite f data) tid
+      fs
+      tt
+      (upd_file f data fs).
 
-  Variable opT : Type -> Type.
-  Variable op_step : OpSemantics opT State.
-  Variable EquivR : Relation_Definitions.relation State.
+  Definition step := xstep.
 
-  Inductive equiv_step : OpSemantics opT State :=
-  | StepEquiv : forall `(op : opT T) tid s0 s1 s1' r,
-    op_step op tid s0 r s1' ->
-    EquivR s1 s1' ->
-    equiv_step op tid s0 r s1.
+End LinkAPI.
 
-End StepXform.
 
-Inductive fs_step : forall T, fsOpT T -> nat -> State -> T -> State -> Prop :=
-| StepCreate : forall dir dirnum name tid s h s',
-  path_eval_root s dir (DirNode dirnum) ->
-  does_not_exist s dirnum name ->
-  file_handle_unused s h ->
-  file_handle_valid s h ->
-  s' = create_file dirnum h name s ->
-  fs_step (Create dir name) tid s h s'
+Notation "x <?- p1 ; p2" := (r <- p1; match r with | None => Ret None | Some x => p2 end)
+  (at level 60, right associativity).
 
-(*
 
-| StepMkdir : forall dir name tid s h s' dirnum newdirnum,
-  frame_pre_post s s'
-    (dir |-> Dir dirnum * (dir ++ [name]) |-> Missing)
-    (dir |-> Dir dirnum * (dir ++ [name]) |-> Dir newdirnum
-                        * subtree_pred (dir ++ [name]) empty_dir) ->
-  fs_step (Mkdir dir name) tid s h s'
+Fixpoint namei_spec (nstep : nat) (startnode : Node) (pn : Pathname) : proc _ (option Node) :=
+  match nstep with
+  | O => Ret None
+  | S nstep' =>
+    match pn with
+    | nil =>
+      Ret (Some startnode)
+    | name :: pn' =>
+      match startnode with
+      | DirNode startdir =>
+        r <- Op (LinkLookup startdir name);
+        match r with
+        | None => Ret None
+        | Some (SymlinkNode sympath) =>
+          osymnode <- namei_spec nstep' startnode sympath;
+          match osymnode with
+          | None => Ret None
+          | Some symnode =>
+            namei_spec nstep' symnode pn'
+          end
+        | Some n =>
+          namei_spec nstep' n pn'
+        end
+      | _ => Ret None
+      end
+    end
+  end.
 
-| StepDelete : forall pn h f tid s s',
-  frame_pre_post s s'
-    (pn |-> File h f)
-    (pn |-> Missing) ->
-  fs_step (Delete pn) tid s tt s'
+Definition namei_cwd (cwd : nat) (pn : Pathname) : proc _ (option Node) :=
+  namei_spec 100 (DirNode cwd) pn.
 
-| StepRmdir : forall pn dirnum tid s s',
-  frame_pre_post s s'
-    (pn |-> Dir dirnum * subtree_pred pn empty_dir)
-    (pn |-> Missing) ->
-  fs_step (Rmdir pn) tid s tt s'
+Definition namei_cwd_dir (cwd : nat) (pn : Pathname) : proc _ (option nat) :=
+  r <?- namei_spec 100 (DirNode cwd) pn;
+  match r with
+  | DirNode dirnum => Ret (Some dirnum)
+  | _ => Ret None
+  end.
 
-| StepStat : forall dir name tid s r F dirnum,
-  s  |= F * dir |-> Dir dirnum ->
-  (r = StatFile ->
-    exists F' h f, F' * (dir ++ [name]) |-> File h f ===> F) ->
-  (r = StatDir ->
-    exists F' dirnum', F' * (dir ++ [name]) |-> Dir dirnum' ===> F) ->
-  (r = StatMissing ->
-    exists F', F' * (dir ++ [name]) |-> Missing ===> F) ->
-  fs_step (Stat dir name) tid s r s
+Definition namei_cwd_file (cwd : nat) (pn : Pathname) : proc _ (option nat) :=
+  r <?- namei_spec 100 (DirNode cwd) pn;
+  match r with
+  | FileNode h => Ret (Some h)
+  | _ => Ret None
+  end.
 
-| StepReaddir : forall dir tid s r F dirnum,
-  s  |= F * dir |-> Dir dirnum ->
-  (forall fn,
-    (In fn r /\ exists F' handle f,
-     F' * (dir ++ [fn]) |-> File handle f ===> F) \/
-    (In fn r /\ exists F' dirinum,
-     F' * (dir ++ [fn]) |-> Dir dirinum ===> F) \/
-    (~ In fn r /\ exists F',
-     F' * (dir ++ [fn]) |-> Missing ===> F)) ->
-  fs_step (Readdir dir) tid s r s
+Definition create (cwd : nat) (dir : Pathname) (name : string) :=
+  dirnum <?- namei_cwd_dir cwd dir;
+  Op (LinkAllocFile dirnum name).
 
-| StepRename : forall src dstdir dstname tid s handle f s' dirnum,
-  frame_pre_post s s'
-    (src |-> File handle f
-          * dstdir |-> Dir dirnum
-          * (dstdir ++ [dstname]) |-> Missing)
-    (src |-> Missing
-          * dstdir |-> Dir dirnum
-          * (dstdir ++ [dstname]) |-> File handle f) ->
-  fs_step (Rename src dstdir dstname) tid s tt s'
+Definition mkdir (cwd : nat) (dir : Pathname) (name : string) :=
+  dirnum <?- namei_cwd_dir cwd dir;
+  Op (LinkAllocDir dirnum name).
 
-| StepRead : forall pn tid s r handle F,
-  s  |= F * pn |-> File handle r ->
-  fs_step (Read pn) tid s (FileData r) s
+Definition unlink (cwd : nat) (dir : Pathname) (name : string) :=
+  dirnum <?- namei_cwd_dir cwd dir;
+  n <?- Op (LinkLookup dirnum name);
+  _ <- Op (LinkDel dirnum name n);
+  Ret (Some tt).
 
-| StepWrite : forall pn tid s s' handle f0 data,
-  frame_pre_post s s'
-    (pn |-> File handle f0)
-    (pn |-> File handle (mk_file data)) ->
-  fs_step (Write pn data) tid s tt s'
+Definition stat (cwd : nat) (dir : Pathname) (name : string) :=
+  dirnum <?- namei_cwd_dir cwd dir;
+  n <?- Op (LinkLookup dirnum name);
+  match n with
+  | FileNode _ => Ret (Some StatFile)
+  | DirNode _ => Ret (Some StatDir)
+  | _ => Ret None
+  end.
 
-| StepFindAvailableName : forall dir dirnum tid s name F,
-  starts_with_tid tid name ->
-  s  |= F * dir |-> Dir dirnum * (dir ++ [name]) |-> Missing ->
-  fs_step (FindAvailableName dir) tid s name s
+Definition readdir (cwd : nat) (pn : Pathname) :=
+  dirnum <?- namei_cwd_dir cwd pn;
+  Op (LinkList dirnum).
 
-| StepDebug : forall msg tid s,
-  fs_step (Debug msg) tid s tt s
-*)
-.
+Definition rename (cwd : nat) (srcdir : Pathname) (srcname : string)
+                              (dstdir : Pathname) (dstname : string) :=
+  srcdirnum <?- namei_cwd_dir cwd srcdir;
+  dstdirnum <?- namei_cwd_dir cwd dstdir;
+  srcnode <?- Op (LinkLookup srcdirnum srcname);
+  dstnodeopt <- Op (LinkLookup dstdirnum dstname);
+  match srcnode with
+  | FileNode _ =>
+    match dstnodeopt with
+    | None =>
+      _ <- Op (LinkAdd dstdirnum dstname srcnode);
+      _ <- Op (LinkDel srcdirnum srcname srcnode);
+      Ret (Some tt)
+    | Some (FileNode dstfile) =>
+      _ <- Op (LinkAdd dstdirnum dstname srcnode);
+      _ <- Op (LinkDel dstdirnum dstname (FileNode dstfile));
+      _ <- Op (LinkDel srcdirnum srcname srcnode);
+      Ret (Some tt)
+    | _ =>
+      Ret None
+    end
+  | _ => Ret None
+  end.
 
-Hint Constructors fs_step.
+Definition read (cwd : nat) (pn : Pathname) :=
+  f <?- namei_cwd_file cwd pn;
+  d <- Op (FileRead f);
+  Ret (Some d).
 
-Definition fs_step_equiv : OpSemantics fsOpT State :=
-  equiv_step fs_step FSEquiv.
-
-Instance fs_step_equiv_proper :
-  Proper (eq ==> eq ==> eq ==> eq ==> FSEquiv ==> iff) (@fs_step_equiv T).
-Proof.
-  intros.
-  intros ? ? ?; subst.
-  intros ? ? ?; subst.
-  intros fs1 fs1' ?.
-  intros ? ? ?; subst.
-  intros fs2 fs2' ?.
-  unfold fs_step_equiv; intuition.
-  - inversion H0; clear H0; repeat sigT_eq.
-    econstructor; eauto.
-    etransitivity; eauto.
-      symmetry; eauto.
-  - inversion H0; clear H0; repeat sigT_eq.
-    econstructor; eauto.
-    etransitivity; eauto.
-Qed.
-
-Instance file_handle_unused_proper :
-  Proper (FSEquiv ==> eq ==> iff) file_handle_unused.
-Proof.
-  intros ? ? ?; subst.
-  intros ? ? ?; subst.
-  unfold FSEquiv in H.
-  unfold file_handle_unused; intuition; repeat deex.
-  - apply H2 in H3. eauto.
-  - apply H2 in H3. eauto.
-Qed.
-
-Instance file_handle_valid_proper :
-  Proper (FSEquiv ==> eq ==> iff) file_handle_valid.
-Proof.
-  intros ? ? ?; subst.
-  intros ? ? ?; subst.
-  unfold FSEquiv in H.
-  unfold file_handle_valid; intuition; congruence.
-Qed.
-
-Instance does_not_exist_proper :
-  Proper (FSEquiv ==> eq ==> eq ==> iff) does_not_exist.
-Proof.
-  intros ? ? ?; subst.
-  intros ? ? ?; subst.
-  intros ? ? ?; subst.
-  unfold FSEquiv in H.
-  unfold does_not_exist; intuition; repeat deex.
-  - apply H2 in H3. eauto.
-  - apply H2 in H3. eauto.
-Qed.
-
-Instance FSEquiv_proper :
-  Proper (FSEquiv ==> FSEquiv ==> iff) FSEquiv.
-Proof.
-  intros ? ? ?; subst.
-  intros ? ? ?; subst.
-  rewrite H. rewrite H0. reflexivity.
-Qed.
-
-Instance upd_file_proper :
-  Proper (eq ==> eq ==> FSEquiv ==> FSEquiv) upd_file.
-Proof.
-  intros ? ? ?; subst.
-  intros ? ? ?; subst.
-  intros ? ? ?; subst.
-  unfold upd_file.
-  unfold FSEquiv in *.
-  intuition; simpl.
-  rewrite H; eauto.
-Qed.
-
-Instance add_link_proper :
-  Proper (eq ==> eq ==> eq ==> FSEquiv ==> FSEquiv) add_link.
-Proof.
-  intros ? ? ?; subst.
-  intros ? ? ?; subst.
-  intros ? ? ?; subst.
-  intros ? ? ?; subst.
-  unfold add_link.
-  unfold FSEquiv in *.
-  intuition; simpl.
-
-  unfold Graph.Equal; split; intros; apply Graph.add_spec.
-  - apply Graph.add_spec in H1; intuition; subst.
-    apply H2 in H3. eauto.
-  - apply Graph.add_spec in H1; intuition; subst.
-    apply H2 in H3. eauto.
-Qed.
-
-Instance create_file_proper :
-  Proper (eq ==> eq ==> eq ==> FSEquiv ==> FSEquiv) create_file.
-Proof.
-  intros ? ? ?; subst.
-  intros ? ? ?; subst.
-  intros ? ? ?; subst.
-  intros ? ? ?; subst.
-  unfold create_file.
-  rewrite H.
-  reflexivity.
-Qed.
-
+Definition write (cwd : nat) (pn : Pathname) (data : string) :=
+  f <?- namei_cwd_file cwd pn;
+  _ <- Op (FileWrite f data);
+  Ret (Some tt).
