src/FS/FSModel.v
@@ -1,0 +1,980 @@
+Require Import POCS.
+Require Import String.
+Require Import Equalities.
+Require Import MSets.MSetWeakList.
+Require Import Relations.Relation_Operators.
+Require Import RelationClasses.
+Require Import Morphisms.
+Require Import Sumbool.
+
+Import ListNotations.
+Open Scope string.
+
+(** Declarative spec for a FS interface with concurrent operations, modeled
+ after POCS notes.  The file system is represented as set of links.  To allow
+ for concurrent operations a directory may contain a link with the same name
+ twice, but for different nodes.  For example, we model a rename as a link
+ followed by an unlink.  Thus, a lookup after link and before unlink may observe
+ a duplicate name, but each name has a different node. *)
+
+
+(** Data types *)
+
+Inductive Node :=
+| DirNode : forall (dirnum : nat), Node
+| FileNode : forall (filenum : nat), Node
+| SymlinkNode : forall (target : list string), Node.
+
+Record Link := mkLink {
+  LinkFrom : nat;   (* Always a DirNode *)
+  LinkTo : Node;
+  LinkName : string
+}.
+
+Instance Node_equal_dec : EqualDec Node.
+  unfold EqualDec; intros.
+  destruct x, y; try (right; congruence).
+  destruct (eq_nat_dec dirnum dirnum0); subst; eauto.
+    right; congruence.
+  destruct (eq_nat_dec filenum filenum0); subst; eauto.
+    right; congruence.
+  destruct (list_eq_dec string_dec target target0); subst; eauto.
+    right; congruence.
+Defined.
+
+Lemma Link_equal_dec : EqualDec Link.
+  unfold EqualDec; intros.
+  destruct x, y.
+  destruct (eq_nat_dec LinkFrom0 LinkFrom1); subst.
+  destruct (Node_equal_dec LinkTo0 LinkTo1); subst.
+  destruct (string_dec LinkName0 LinkName1); subst.
+  eauto.
+  right; congruence.
+  right; congruence.
+  right; congruence.
+Defined.
+
+Module MDT_Link.
+  Definition t := Link.
+  Definition eq_dec := Link_equal_dec.
+End MDT_Link.
+
+Module Link_as_UDT := Make_UDT(MDT_Link).
+
+Module Graph := MSetWeakList.Make Link_as_UDT.
+
+Definition eq_string (s1 s2 : string) :=
+  if string_dec s1 s2 then true else false.
+
+Definition proper_nameb n : bool := negb (orb (eq_string n  ".") (eq_string n "..")).
+Definition proper_name n := n <> "." /\ n <> "..".
+Definition proper_link l := proper_name (LinkName l).
+Definition proper_links g := Graph.For_all proper_link g.
+Instance proper_proper_link:
+  Proper (eq ==> eq) proper_link.
+Proof.
+  intros ? ?.
+  intros; subst; reflexivity.
+Qed.
+
+Lemma In_add_add_comm: forall a l1 l2 g,
+    Graph.In a (Graph.add l1 (Graph.add l2 g)) ->
+    Graph.In a (Graph.add l2 (Graph.add l1 g)).
+Proof.
+  intros.
+  eapply Graph.add_spec in H; intuition idtac; subst.
+  eapply Graph.add_spec; right. eapply Graph.add_spec; eauto.
+  eapply Graph.add_spec in H0; intuition idtac; subst.
+  eapply Graph.add_spec; eauto.
+  eapply Graph.add_spec; right. eapply Graph.add_spec; eauto.
+Qed.
+
+Definition File := string.
+Definition Files := list File.
+
+Record FS := mkFS {
+  FSRoot : nat;     (* root DirNode *)
+  FSLinks : Graph.t;
+  FSFiles : Files;  (* [filenum]s point into this list *)
+}.
+
+Definition Pathname := list string.
+
+Definition FSEquiv (fs1 fs2 : FS) : Prop :=
+  FSRoot fs1 = FSRoot fs2 /\
+  FSFiles fs1 = FSFiles fs2 /\
+  Graph.Equal (FSLinks fs1) (FSLinks fs2).
+
+Instance FSEquiv_Equiv : Equivalence FSEquiv.
+Proof.
+  split; unfold FSEquiv.
+  - intros f; intuition eauto.
+    reflexivity.
+  - intros f1 f2; intuition eauto.
+    symmetry. eauto.
+  - intros f1 f2 f3; intuition eauto.
+    congruence.
+    congruence.
+    etransitivity; eauto.
+Qed.
+
+Ltac subst_fsequiv :=
+  match goal with
+  | H : FSEquiv ?s1 ?s2 |- _ =>
+    idtac "substituting" s1 "using" H; rewrite H in *; clear H; clear s1;
+    idtac "cleared" s1
+  | H : FSEquiv ?s1 ?s2 |- _ =>
+    idtac "substituting" s2 "using" H; rewrite <- H in *; clear H; clear s2;
+    idtac "cleared" s2
+  end.
+
+(** [path_evaluates] is used to specify lookup *)
+
+Inductive valid_link : forall (fs : FS) (dir : nat) (name : string) (target : Node), Prop :=
+| ValidLink : forall fs dir name target,
+(*
+    proper_name name ->
+    (exists parent name,
+        Graph.In (mkLink parent (DirNode dir) name) (FSLinks fs) ->
+        target <> DirNode parent) ->
+*)
+    Graph.In (mkLink dir target name) (FSLinks fs) ->
+    valid_link fs dir name target
+| ValidDot : forall fs dir,
+    valid_link fs dir "." (DirNode dir)
+| ValidDotDot : forall fs dir name parent,
+    Graph.In (mkLink parent (DirNode dir) name) (FSLinks fs) ->
+    valid_link fs dir ".." (DirNode parent)
+| ValidDotDotRoot : forall fs dir,
+    dir = FSRoot fs ->
+    valid_link fs dir ".." (DirNode dir).
+
+Instance valid_link_proper :
+  Proper (FSEquiv ==> eq ==> eq ==> eq ==> iff) valid_link.
+Proof.
+  intros fs1 fs2 H.
+  intros ? ? ?; subst.
+  intros ? ? ?; subst.
+  intros ? ? ?; subst.
+  unfold FSEquiv in H; intuition idtac.
+  - inversion H1.
+    + eapply ValidLink.
+      eapply H2; eauto.
+    + eapply ValidDot.
+    + eapply ValidDotDot.
+      eapply H2; eauto.
+    + eapply ValidDotDotRoot. congruence.
+  - inversion H1.
+    + eapply ValidLink.
+      eapply H2; eauto.
+    + eapply ValidDot.
+    + eapply ValidDotDot.
+      eapply H2; eauto.
+    + eapply ValidDotDotRoot. congruence.
+Qed.
+
+Definition proper_link' fs l := proper_name (LinkName l) /\
+                             (exists parent, valid_link fs (LinkFrom l) ".." parent ->
+                                (LinkTo l) <> parent).
+
+Inductive path_evaluates : forall (fs : FS) (start : Node) (pn : Pathname) (target : Node), Prop :=
+| PathEvalEmpty : forall fs start,
+  path_evaluates fs start nil start
+| PathEvalFileLink : forall fs startdir name inum,
+  valid_link fs startdir name (FileNode inum)  ->
+  path_evaluates fs (DirNode startdir) ([name]) (FileNode inum)
+| PathEvalDirLink : forall fs startdir name inum pn namenode,
+  valid_link fs startdir name (DirNode inum) ->
+  path_evaluates fs (DirNode inum) pn namenode ->
+  path_evaluates fs (DirNode startdir) (name :: pn) namenode
+| PathEvalSymlink : forall fs startdir name sympath symtarget pn target,
+  valid_link fs startdir name (SymlinkNode sympath) ->
+  path_evaluates fs (DirNode startdir) sympath symtarget ->
+  path_evaluates fs symtarget pn target ->
+  path_evaluates fs (DirNode startdir) (name :: pn) target.
+
+Instance path_evaluates_proper :
+  Proper (FSEquiv ==> eq ==> eq ==> eq ==> iff) path_evaluates.
+Proof.
+  intros fs1 fs2 H.
+  intros ? ? ?; subst.
+  intros ? ? ?; subst.
+  intros ? ? ?; subst.
+  intuition.
+  - induction H0.
+    + eapply PathEvalEmpty.
+    + eapply PathEvalFileLink; eauto.
+      rewrite H in H0. eauto.
+    + eapply PathEvalDirLink; eauto.
+      rewrite H in H0. eauto.
+    + eapply PathEvalSymlink; eauto.
+      rewrite H in H0; eauto.
+  - induction H0.
+    + eapply PathEvalEmpty.
+    + eapply PathEvalFileLink; eauto.
+      rewrite <- H in H0. eauto.
+    + eapply PathEvalDirLink; eauto.
+      rewrite <- H in H0. eauto.
+    + eapply PathEvalSymlink; eauto.
+      rewrite <- H in H0; eauto.
+Qed.
+
+Definition path_eval_root (fs : FS) (pn : Pathname) (target : Node) : Prop :=
+  path_evaluates fs (DirNode (FSRoot fs)) pn target.
+
+Instance path_eval_root_proper :
+  Proper (FSEquiv ==> eq ==> eq ==> iff) path_eval_root.
+Proof.
+  intros fs1 fs2 H.
+  intros ? ? ?; subst.
+  intros ? ? ?; subst.
+  unfold path_eval_root.
+  eapply path_evaluates_proper; eauto.
+  unfold FSEquiv in *; intuition.
+Qed.
+
+Hint Constructors valid_link.
+Hint Constructors path_evaluates.
+
+Lemma path_evaluates_cons': forall fs startdir name pn node,
+    path_evaluates fs startdir (name::pn) node ->
+    exists node',
+      path_evaluates fs startdir [name] node' /\
+      path_evaluates fs node' pn node.
+Proof.
+  intros.
+  inversion H; subst; eexists; eauto.
+Qed.
+
+Lemma path_evaluates_cons: forall fs startdir name pn node node',
+    path_evaluates fs (DirNode startdir) [name] node' ->
+    path_evaluates fs node' pn node ->
+    exists node'',
+      path_evaluates fs (DirNode startdir) (name::pn) node''.
+Proof.
+  intros.
+  inversion H; subst; clear H.
+  - eexists.
+    inversion H0; subst; clear H0.
+    constructor; eauto.
+  - eexists.
+    eapply PathEvalDirLink; eauto.
+    inversion H7; subst; clear H7.
+    eauto.
+  - eexists.
+    inversion H8; subst; clear H8.
+    eapply PathEvalSymlink; eauto.
+Qed.
+
+Definition does_not_exist (fs : FS) dirnum name :=
+  ~ exists n, Graph.In (mkLink dirnum n name) (FSLinks fs).
+
+Definition file_handle_unused (fs : FS) h :=
+  ~ exists d name, Graph.In (mkLink d (FileNode h) name) (FSLinks fs).
+
+Definition file_handle_valid (fs : FS) h :=
+  h < Datatypes.length (FSFiles fs).
+
+Definition upd_file h data (fs : FS) :=
+  mkFS (FSRoot fs) (FSLinks fs) (list_upd (FSFiles fs) h data).
+
+Definition add_link dir node name (fs : FS) :=
+  mkFS (FSRoot fs) (Graph.add (mkLink dir node name) (FSLinks fs)) (FSFiles fs).
+
+Definition del_link dir node name (fs : FS) :=
+  mkFS (FSRoot fs) (Graph.remove (mkLink dir node name) (FSLinks fs)) (FSFiles fs).
+
+Definition create_file dir h name (fs : FS) :=
+  add_link dir (FileNode h) name (upd_file h "" fs).
+
+Definition valid_dir dir (fs : FS) :=
+  exists pn, path_eval_root fs pn (DirNode dir).
+
+Definition match_readdir from l :=
+  beq_nat from (LinkFrom l).
+
+Definition readdir fs dir :=
+  Graph.filter (match_readdir dir) (FSLinks fs).
+
+Definition readdir_names fs dir :=
+  map LinkName (Graph.elements (readdir fs dir)).
+
+(* If pn exists, then it is unique. *)
+Definition unique_pathname (fs : FS) startdir pn :=
+  exists node,
+    path_evaluates fs startdir pn node /\
+    forall node',
+      path_evaluates fs startdir pn node' -> node' = node.
+
+Definition unique_pathname_root (fs : FS) pn :=
+  exists node,
+    path_eval_root fs pn node /\
+    forall node',
+      path_eval_root fs pn node' -> node' = node.
+
+Lemma unique_pathname_path_evaluates_eq: forall fs startdir pn node node',
+    unique_pathname fs startdir pn ->
+    path_evaluates fs startdir pn node ->
+    path_evaluates fs startdir pn node' ->
+    node = node'.
+Proof.
+  intros.
+  unfold unique_pathname in *.
+  deex.
+  specialize (H2 node H0) as H2x; subst.
+  specialize (H2 node' H1) as H2x; subst.
+  reflexivity.
+Qed.
+
+Lemma unique_pathname_valid_link_eq: forall fs dirnum name inum inum',
+    unique_pathname fs (DirNode dirnum) [name] ->
+    valid_link fs dirnum name (DirNode inum) ->
+    valid_link fs dirnum name (DirNode inum') ->
+    DirNode inum = DirNode inum'.
+Proof.
+  intros.
+  unfold unique_pathname in *.
+  deex.
+  specialize (H2 (DirNode inum)) as H2x; subst.
+  specialize (H2 (DirNode inum')) as H2y; subst.
+  destruct H2x.
+  econstructor.
+  eapply H0.
+  constructor.
+  destruct H2y.
+  econstructor.
+  eapply H1.
+  constructor.
+  reflexivity.
+Qed.
+
+Lemma unique_pathname_path_evaluates_cons_eq: forall fs startdir name pn' node node' node'',
+    path_evaluates fs (DirNode startdir) [name] node' ->
+    path_evaluates fs node' pn' node ->
+    unique_pathname fs (DirNode startdir) [name] ->
+    unique_pathname fs node' pn' ->
+    path_evaluates fs (DirNode startdir) (name :: pn') node'' ->
+    node = node''.
+Proof.
+  intros.
+  eapply path_evaluates_cons' in H3 as Hcons.
+  deex.
+  assert (node'0 = node').
+  eapply unique_pathname_path_evaluates_eq in H; eauto.
+  subst.
+  assert (node = node'').
+  eapply unique_pathname_path_evaluates_eq in H2; eauto.
+  subst.
+  reflexivity.
+Qed.
+
+(* A stronger version of unique_pathname, requiring all intermediate nodes match *)
+Inductive stable_pathname : forall (fs: FS) (startdir: Node) (pn: Pathname), Prop :=
+| StablePathNil: forall fs startdir, stable_pathname fs (DirNode startdir) []
+| StablePathCons: forall fs startdir name pn' node node',
+    path_evaluates fs (DirNode startdir) [name] node' ->
+    path_evaluates fs node' pn' node ->
+    unique_pathname fs (DirNode startdir) [name] ->
+    unique_pathname fs node' pn' ->
+    stable_pathname fs (DirNode startdir) (name::pn').
+
+(* sanity check *)
+Lemma stable_pathname_unique_pathname: forall fs startdir pn,
+    stable_pathname fs startdir pn ->
+    unique_pathname fs startdir pn.
+Proof.
+  intros.
+  inversion H; subst; clear H.
+  - eexists.
+    split.
+    constructor.
+    intros.
+    inversion H; auto.
+  - unfold unique_pathname.
+    eapply path_evaluates_cons in H1 as Hcons; eauto.
+    deex.
+    eapply unique_pathname_path_evaluates_cons_eq in H as Hx; eauto.
+    subst.
+    exists node''.
+    split; eauto.
+    intros.
+    eapply unique_pathname_path_evaluates_cons_eq in H4 as Hx; eauto.
+Qed.
+                               
+Definition unique_dirent (fs : FS) dir name :=
+  forall target target0,
+    valid_link fs dir name target ->
+    valid_link fs dir name target0 ->
+    target0 = target.
+
+Definition unique_dirents (fs : FS) :=
+  forall dir name target target0,
+    valid_link fs dir name target ->
+    valid_link fs dir name target0 ->
+    target0 = target.
+
+Lemma unique_dirent_link_eq: forall fs startdir name node node',
+    unique_dirent fs startdir name ->
+    valid_link fs startdir name node ->
+    valid_link fs startdir name node' ->
+    node = node'.
+Proof.
+  intros.
+  edestruct H; eauto.
+Qed.
+
+(* . and .. are unique; which we get from definition.
+  no other name in directory refers to parent or cur directory *)
+
+Definition fs_invariant (fs : FS) := proper_links (FSLinks fs).
+
+(*
+Definition unique_dotdot (fs : FS) :=
+
+                  
+Definition fs_invariant1 (fs : FS) := proper_links (FSLinks fs) /\
+                                      unique_dotdot.
+*)
+
+Lemma fs_invariant_proper_name: forall fs startdir node name,
+    fs_invariant fs ->
+    Graph.In (mkLink startdir node name) (FSLinks fs) ->
+    proper_name name.
+Proof.
+  intros.
+  unfold fs_invariant in *.
+  unfold proper_links in *.
+  unfold Graph.For_all in *.
+  specialize (H (mkLink startdir node name) H0); eauto.
+Qed.
+
+Lemma fs_invariant_add_link: forall fs dirnum name node,
+    fs_invariant fs ->
+    proper_name name ->
+    does_not_exist fs dirnum name ->
+    fs_invariant (add_link dirnum node name fs).
+Proof.
+  intros.
+  unfold fs_invariant in *.
+  unfold proper_links in *.
+  unfold proper_link in *.
+  unfold Graph.For_all in *.
+  intros; simpl in *.
+  eapply Graph.add_spec in H2; eauto.
+  intuition idtac; subst; simpl in *; eauto.
+Qed.
+
+Lemma path_evaluates_add_link : forall fs startdir dirnum name dirpn n node,
+  path_evaluates fs startdir dirpn node ->
+  path_evaluates (add_link dirnum n name fs) startdir dirpn node.
+Proof.
+  unfold add_link in *.
+  simpl in *.
+  intros.
+  induction H.
+  + constructor.
+  + eapply PathEvalFileLink; eauto.
+    edestruct H.
+    - constructor; simpl.
+      apply Graph.add_spec; auto.
+    - apply ValidDot.
+    - eapply ValidDotDot.
+      apply Graph.add_spec; auto.
+      right; eauto.
+    - apply ValidDotDotRoot; auto.
+  + eapply PathEvalDirLink; eauto.
+    edestruct H.
+    - constructor; simpl.
+      apply Graph.add_spec; auto.
+    - apply ValidDot.
+    - eapply ValidDotDot.
+      apply Graph.add_spec; auto.
+      right; eauto.
+    - apply ValidDotDotRoot; auto.
+  + inversion H; subst.
+    eapply PathEvalSymlink; simpl.
+    - constructor.
+      apply Graph.add_spec.
+      eauto.
+    - apply IHpath_evaluates1; eauto.
+    - apply IHpath_evaluates2; eauto.
+Qed.
+
+Lemma valid_link_does_not_exist: forall fs dirnum name node,
+    proper_name name ->
+    valid_link fs dirnum name node ->
+    does_not_exist fs dirnum name ->
+    False.
+Proof.
+  intros.
+  inversion H0; subst; clear H0.
+  - destruct H1; eexists; eauto.
+  - destruct H; congruence.
+  - destruct H; congruence.
+  - destruct H; congruence.
+Qed.
+
+Lemma path_evaluates_does_not_exist: forall fs dirnum name,
+    proper_name name ->
+    path_evaluates fs (DirNode dirnum) [name] (DirNode dirnum) ->
+    does_not_exist fs dirnum name ->
+    False.
+Proof.
+  intros.
+  inversion H0; subst; clear H0.
+  inversion H8; subst; clear H8.
+  eapply valid_link_does_not_exist; eauto.
+  inversion H9; subst; clear H9.
+  eapply valid_link_does_not_exist; eauto.
+Qed.
+
+Lemma valid_link_add_link': forall fs startdir name name0 dirnum n node node',
+    proper_name name0 ->
+    valid_link fs startdir name0 node ->
+    proper_name name  ->
+    does_not_exist fs dirnum name ->
+    valid_link (add_link dirnum n name fs) startdir name0 node' ->
+    valid_link fs startdir name0 node'.
+Proof.
+  intros.
+  inversion H3; subst; clear H3.
+  - apply Graph.add_spec in H4.
+    intuition idtac; auto.
+    inversion H3; subst; clear H3.
+    exfalso; eapply valid_link_does_not_exist; eauto.
+  - apply ValidDot.
+  - eapply ValidDotDot.
+    apply Graph.add_spec in H4; auto.
+    intuition idtac; eauto.
+    inversion H3; subst. clear H3.
+    inversion H; congruence.
+  - eapply ValidDotDotRoot.
+    simpl in *.
+    reflexivity.
+Qed. 
+
+Lemma valid_link_add_link'': forall fs startdir name name0 dirnum n node node',
+    valid_link fs startdir name0 node ->
+    proper_name name  ->
+    does_not_exist fs dirnum name ->
+    valid_link (add_link dirnum n name fs) startdir name0 node' ->
+    valid_link fs startdir name0 node'.
+Proof.
+  intros.
+  inversion H2; subst; clear H2.
+  - apply Graph.add_spec in H3.
+    intuition idtac; auto.
+    inversion H2; subst; clear H2.
+    exfalso; eapply valid_link_does_not_exist; eauto.
+  - apply ValidDot.
+  - eapply ValidDotDot.
+    apply Graph.add_spec in H3; auto.
+    intuition idtac; eauto.
+    inversion H2; subst. clear H2.
+    admit. 
+  - eapply ValidDotDotRoot.
+    simpl in *.
+    reflexivity.
+Admitted. 
+
+Lemma path_evaluates_add_link' : forall fs startdir dirnum name dirpn n node,
+  fs_invariant fs ->
+  stable_pathname fs startdir dirpn ->
+  path_evaluates fs startdir dirpn (DirNode dirnum) ->
+  does_not_exist fs dirnum name  ->
+  proper_name name ->
+  path_evaluates (add_link dirnum n name fs) startdir dirpn node ->
+  path_evaluates fs startdir dirpn node.
+Proof.
+  intros.
+  remember (add_link dirnum n name fs).
+  generalize dependent fs; intros.
+  induction H4; subst.
+  - constructor.
+  - eapply PathEvalFileLink; subst; eauto.
+    inversion H4; subst.
+    eapply fs_invariant_proper_name in H5 as H5x.
+    eapply Graph.add_spec in H5.
+    intuition idtac.
+    + inversion H6; subst; clear H6.
+      eapply path_evaluates_does_not_exist in H2; eauto.
+      exfalso; auto.
+    + constructor; eauto.
+    + apply fs_invariant_add_link; eauto.
+  - inversion H1; subst; clear H1.
+    {
+      eapply PathEvalDirLink; eauto.
+      eapply valid_link_add_link'' in H4; auto.
+      assert (DirNode inum0 = DirNode inum).
+      {
+        inversion H0; subst.
+        eapply unique_pathname_valid_link_eq.
+        eapply H13.
+        eauto.
+        eauto.
+      }
+      inversion H1; subst; clear H1.
+      eapply IHpath_evaluates; eauto.
+      admit.
+      eauto.
+    }
+    {
+      inversion H10; subst.
+      eapply fs_invariant_proper_name in H1 as Hx; eauto.
+      eapply valid_link_add_link'' in H4; eauto.
+      exfalso. admit. (* H2 + H8 + H *)
+    }
+  - eapply PathEvalSymlink; eauto; subst.
+    inversion H0; subst.
+    (*
+    - constructor.
+      apply Graph.add_spec.
+      eauto.
+    - apply IHpath_evaluates1; eauto.
+    - apply IHpath_evaluates2; eauto.
+*)
+Admitted.
+
+Lemma path_eval_root_add_link : forall fs dirnum name dirpn n,
+  path_eval_root fs dirpn (DirNode dirnum) ->
+  path_eval_root (add_link dirnum n name fs) dirpn (DirNode dirnum).
+Proof.
+  intros.
+  unfold path_eval_root.
+  eapply path_evaluates_add_link in H; eauto.
+Qed.
+
+Lemma path_evaluates_upd_file : forall fs startdir dirnum h data dirpn,
+  path_evaluates fs startdir dirpn (DirNode dirnum) ->
+  path_evaluates (upd_file h data fs) startdir dirpn (DirNode dirnum).
+Proof.
+  intros.
+  unfold upd_file; simpl.
+  induction H.
+  + constructor.
+  + eapply PathEvalFileLink; eauto.
+    edestruct H.
+    - constructor; simpl; auto.
+    - apply ValidDot.
+    - eapply ValidDotDot; simpl; eauto.
+    - apply ValidDotDotRoot; auto.
+  + eapply PathEvalDirLink; eauto.
+    edestruct H.
+    - constructor; simpl; auto.
+    - apply ValidDot.
+    - eapply ValidDotDot; simpl; eauto.
+    - apply ValidDotDotRoot; auto.
+  + eapply PathEvalSymlink; simpl.
+    inversion H. constructor. eauto.
+    apply IHpath_evaluates1; eauto.
+    apply IHpath_evaluates2; eauto.
+Qed.
+
+Lemma path_eval_root_upd_file : forall fs dirnum h data dirpn,
+  path_eval_root fs dirpn (DirNode dirnum) ->
+  path_eval_root (upd_file h data fs) dirpn (DirNode dirnum).
+Proof.
+  intros.
+  unfold path_eval_root in *.
+  eapply path_evaluates_upd_file in H; eauto.
+Qed.
+
+Lemma path_evaluates_upd_file' : forall fs node h data dirpn startdir,
+  path_evaluates (upd_file h data fs) startdir dirpn node ->
+  path_evaluates fs startdir dirpn node.
+Proof.
+  intros.
+  match goal with
+  | H : path_evaluates ?fs0 ?dir0 ?pn0 ?node0 |- _ =>
+    remember fs0;
+    induction H; intros; subst; simpl
+  end.
+  + constructor.
+  + eapply PathEvalFileLink; eauto.
+    inversion H; clear H; subst.
+    constructor. eauto.
+  + eapply PathEvalDirLink; eauto.
+    inversion H; clear H; subst.
+    - constructor. eauto.
+    - apply ValidDot.
+    - eapply ValidDotDot; simpl; eauto.
+    - apply ValidDotDotRoot; auto.
+  + eapply PathEvalSymlink; simpl.
+    inversion H; clear H; subst.
+    constructor; eauto.
+    eapply IHpath_evaluates1; eauto.
+    apply IHpath_evaluates2; eauto.
+Qed.
+
+Lemma path_eval_root_upd_file' : forall fs node h data dirpn,
+  path_eval_root (upd_file h data fs) dirpn node ->
+  path_eval_root fs dirpn node.
+Proof.
+  intros.
+  eapply path_evaluates_upd_file'; eauto.
+Qed.
+
+Lemma does_not_exist_add_link : forall fs dirnum name dirnum0 n0 name0,
+  does_not_exist (add_link dirnum0 n0 name0 fs) dirnum name ->
+  does_not_exist fs dirnum name.
+Proof.
+  intros.
+  unfold does_not_exist, add_link in *.
+  simpl in *.
+  intro.
+  destruct H.
+  deex.
+  eexists.
+  apply Graph.add_spec. right.
+  apply H.
+Qed.
+  
+Lemma does_not_exist_add_link_same_dirnum : forall fs dirnum name n0 name0,
+  does_not_exist fs dirnum name ->
+  name <> name0 ->
+  does_not_exist (add_link dirnum n0 name0 fs) dirnum name.
+Proof.
+  intros.
+  unfold does_not_exist, add_link in *.
+  simpl in *.
+  intro.
+  deex.
+  apply Graph.add_spec in H1.
+  intuition idtac.
+  inversion H2; congruence.
+  destruct H.
+  eexists.
+  apply H2.
+Qed.
+  
+Lemma does_not_exist_upd_file : forall fs h data dirnum name,
+  does_not_exist (upd_file h data fs) dirnum name ->
+  does_not_exist fs dirnum name.
+Proof.
+  intros.
+  unfold does_not_exist, upd_file in *.
+  simpl in *; auto.
+Qed.
+
+Lemma does_not_exist_upd_file' : forall fs h data dirnum name,
+  does_not_exist fs dirnum name ->
+  does_not_exist (upd_file h data fs) dirnum name.
+Proof.
+  intros.
+  unfold does_not_exist, upd_file in *.
+  simpl in *; auto.
+Qed.
+  
+Hint Resolve does_not_exist_add_link.
+Hint Resolve does_not_exist_add_link_same_dirnum.
+Hint Resolve does_not_exist_upd_file.
+Hint Resolve does_not_exist_upd_file'.
+
+Lemma file_handle_unused_upd_file : forall fs h0 data0 h,
+  file_handle_unused (upd_file h0 data0 fs) h ->
+  file_handle_unused fs h.
+Proof.
+  intros.
+  unfold file_handle_unused, upd_file in *.
+  simpl in *; auto.
+Qed.
+
+Lemma file_handle_unused_add_link : forall fs dirnum n name h,
+  file_handle_unused (add_link dirnum n name fs) h ->
+  file_handle_unused fs h.
+Proof.
+  intros.
+  unfold file_handle_unused, add_link in *.
+  simpl in *.
+  intro.
+  repeat deex.
+  destruct H.
+  repeat eexists.
+  apply Graph.add_spec.
+  right. apply H0.
+Qed.
+  
+Lemma file_handle_unused_upd_file' : forall fs h0 data0 h,
+  file_handle_unused fs h ->
+  file_handle_unused (upd_file h0 data0 fs) h.
+Proof.
+  intros.
+  unfold file_handle_unused, upd_file in *.
+  simpl in *; auto.
+Qed.
+
+Lemma file_handle_unused_add_link' : forall fs dirnum n name h,
+  file_handle_unused fs h ->
+  n <> FileNode h ->
+  file_handle_unused (add_link dirnum n name fs) h.
+Proof.
+  intros.
+  unfold file_handle_unused, add_link in *.
+  simpl in *.
+  intro.
+  repeat deex.
+  apply Graph.add_spec in H1.
+  intuition idtac.
+  inversion H2; congruence.
+  destruct H.
+  repeat eexists.
+  apply H2.
+Qed.
+  
+Lemma file_handle_unused_ne : forall fs dirnum v0 v1 name,
+  file_handle_unused (add_link dirnum (FileNode v0) name fs) v1 ->
+  FileNode v1 <> FileNode v0.
+Proof.
+  intros.
+  unfold file_handle_unused, add_link in *.
+  simpl in *.
+  intro.
+  destruct H.
+  repeat eexists.
+  apply Graph.add_spec.
+  left. rewrite H0; eauto.
+Qed.
+
+Hint Resolve file_handle_unused_upd_file.
+Hint Resolve file_handle_unused_add_link.
+Hint Resolve file_handle_unused_add_link'.
+Hint Resolve file_handle_unused_ne.
+
+Lemma file_handle_valid_upd_file : forall fs h0 data0 h,
+  file_handle_valid (upd_file h0 data0 fs) h ->
+  file_handle_valid fs h.
+Proof.
+  intros.
+  unfold file_handle_valid, file_handle_valid, upd_file in *.
+  simpl in *.
+  rewrite length_list_upd in H; auto.
+Qed.
+
+Lemma file_handle_valid_add_link : forall fs dirnum n name h,
+  file_handle_valid (add_link dirnum n name fs) h ->
+  file_handle_valid fs h.
+Proof.
+  intros.
+  unfold file_handle_valid, file_handle_valid, add_link in *.
+  simpl in *; auto.
+Qed.
+
+Lemma file_handle_valid_upd_file' : forall fs h0 data0 h,
+  file_handle_valid fs h ->
+  file_handle_valid (upd_file h0 data0 fs) h.
+Proof.
+  intros.
+  unfold file_handle_valid, file_handle_valid, upd_file in *.
+  simpl in *.
+  rewrite length_list_upd; auto.
+Qed.
+  
+Lemma file_handle_valid_add_link' : forall fs dirnum n name h,
+  file_handle_valid fs h ->
+  file_handle_valid (add_link dirnum n name fs) h.
+Proof.
+  intros.
+  unfold file_handle_valid, file_handle_valid, add_link in *.
+  simpl in *; auto.
+Qed.
+  
+Hint Resolve file_handle_valid_upd_file.
+Hint Resolve file_handle_valid_add_link.
+Hint Resolve file_handle_valid_upd_file'.
+Hint Resolve file_handle_valid_add_link'.
+
+Lemma valid_link_upd_file' : forall fs h data dir name target,
+  valid_link (upd_file h data fs) dir name target ->
+  valid_link fs dir name target.
+Proof.
+  intros.
+  remember (upd_file h data fs); generalize dependent fs.
+  induction H; intros; subst.
+  - constructor. eauto.
+  - eapply ValidDot.
+  - eapply ValidDotDot. eauto.
+  - eapply ValidDotDotRoot. eauto.
+Qed.
+
+Instance file_handle_unused_proper :
+  Proper (FSEquiv ==> eq ==> iff) file_handle_unused.
+Proof.
+  intros ? ? ?; subst.
+  intros ? ? ?; subst.
+  unfold FSEquiv in H.
+  unfold file_handle_unused; intuition; repeat deex.
+  - apply H2 in H3. eauto.
+  - apply H2 in H3. eauto.
+Qed.
+
+Instance file_handle_valid_proper :
+  Proper (FSEquiv ==> eq ==> iff) file_handle_valid.
+Proof.
+  intros ? ? ?; subst.
+  intros ? ? ?; subst.
+  unfold FSEquiv in H.
+  unfold file_handle_valid; intuition; congruence.
+Qed.
+
+Instance does_not_exist_proper :
+  Proper (FSEquiv ==> eq ==> eq ==> iff) does_not_exist.
+Proof.
+  intros ? ? ?; subst.
+  intros ? ? ?; subst.
+  intros ? ? ?; subst.
+  unfold FSEquiv in H.
+  unfold does_not_exist; intuition; repeat deex.
+  - apply H2 in H3. eauto.
+  - apply H2 in H3. eauto.
+Qed.
+
+Instance FSEquiv_proper :
+  Proper (FSEquiv ==> FSEquiv ==> iff) FSEquiv.
+Proof.
+  intros ? ? ?; subst.
+  intros ? ? ?; subst.
+  rewrite H. rewrite H0. reflexivity.
+Qed.
+
+Instance upd_file_proper :
+  Proper (eq ==> eq ==> FSEquiv ==> FSEquiv) upd_file.
+Proof.
+  intros ? ? ?; subst.
+  intros ? ? ?; subst.
+  intros ? ? ?; subst.
+  unfold upd_file.
+  unfold FSEquiv in *.
+  intuition; simpl.
+  rewrite H; eauto.
+Qed.
+
+Instance add_link_proper :
+  Proper (eq ==> eq ==> eq ==> FSEquiv ==> FSEquiv) add_link.
+Proof.
+  intros ? ? ?; subst.
+  intros ? ? ?; subst.
+  intros ? ? ?; subst.
+  intros ? ? ?; subst.
+  unfold add_link.
+  unfold FSEquiv in *.
+  intuition; simpl.
+
+  unfold Graph.Equal; split; intros; apply Graph.add_spec.
+  - apply Graph.add_spec in H1; intuition; subst.
+    apply H2 in H3. eauto.
+  - apply Graph.add_spec in H1; intuition; subst.
+    apply H2 in H3. eauto.
+Qed.
+
+Instance create_file_proper :
+  Proper (eq ==> eq ==> eq ==> FSEquiv ==> FSEquiv) create_file.
+Proof.
+  intros ? ? ?; subst.
+  intros ? ? ?; subst.
+  intros ? ? ?; subst.
+  intros ? ? ?; subst.
+  unfold create_file.
+  rewrite H.
+  reflexivity.
+Qed.
+
