src/POCS.v
@@ -31,3 +31,4 @@ Require Export Spec.ConcurProc.
 Require Export Spec.Equiv.
 Require Export Spec.Compile.
 Require Export Spec.Abstraction.
+Require Export Spec.Modules.
